src/ReactorModel/Components/Update.lean
@@ -120,7 +120,7 @@ notation σ₁:max " -[" cmp ":" i:max f "]→ " σ₂:max => Reactor.Update cmp
 
 theorem Update.requires_lineage_to_target {σ₁ σ₂ : Reactor} {cmp : Cmp} {i : ID} {u : cmp.type → cmp.type → Prop} (h : σ₁ -[cmp;i u]→ σ₂) : Nonempty (Lineage σ₁ cmp i) := by
   induction h
-  case top ha _ _ => exact ⟨Lineage.end cmp $ Finmap.ids_def'.mpr ⟨_, ha⟩⟩
+  case top ha _ _ => exact ⟨Lineage.end cmp $ Finmap.mem_ids_iff.mpr ⟨_, ha⟩⟩
   case nest hn _ _ hi => exact ⟨Lineage.nest hi.some hn⟩
 
 theorem Update.obj?_target {σ₁ σ₂ : Reactor} {cmp : Cmp} {i : ID} {u : cmp.type → cmp.type → Prop} (h : σ₁ -[cmp;i u]→ σ₂) : ∃ o, σ₁.obj? cmp i = some o := by
@@ -128,7 +128,7 @@ theorem Update.obj?_target {σ₁ σ₂ : Reactor} {cmp : Cmp} {i : ID} {u : cmp
 
 theorem Update.preserves_lineage_to_target {σ₁ σ₂ : Reactor} {cmp : Cmp} {i : ID} {u : cmp.type → cmp.type → Prop} (h : σ₁ -[cmp;i u]→ σ₂) : Nonempty (Lineage σ₂ cmp i) := by
   induction h
-  case top ha _ => exact ⟨Lineage.end cmp $ Finmap.ids_def'.mpr ⟨_, ha⟩⟩
+  case top ha _ => exact ⟨Lineage.end cmp $ Finmap.mem_ids_iff.mpr ⟨_, ha⟩⟩
   case nest hn _ hi => exact ⟨Lineage.nest hi.some hn⟩
 
 theorem Update.unique {σ σ₁ σ₂ : Reactor} {cmp : Cmp} {i : ID} {u : cmp.type → cmp.type → Prop} :
@@ -152,7 +152,7 @@ theorem Update.unique {σ σ₁ σ₂ : Reactor} {cmp : Cmp} {i : ID} {u : cmp.t
     rw [hj] at he₁ hn₂
     exact EqModID.eq_from_eq_val_for_id he₁ he₂ hn₂
   case' top.nest σ₁ _ _ _ _ ht _ _ _ _ _ hu hn _ _, nest.top σ₁ _ _ _ _ _ hn _ hu _ _ _ _ ht _ _ =>
-    let l₁ := Lineage.end cmp $ Finmap.ids_def'.mpr ⟨_, ht⟩
+    let l₁ := Lineage.end cmp $ Finmap.mem_ids_iff.mpr ⟨_, ht⟩
     let l₂ := Lineage.nest hu.requires_lineage_to_target.some hn
     have hc := σ₁.uniqueIDs l₁ l₂
     cases cmp <;> contradiction
@@ -185,12 +185,12 @@ theorem Update.compose {σ σ₁ σ₂ : Reactor} {cmp : Cmp} {i : ID} {u₁ u�
     rw [hv₂] at hu₁
     exact Update.top (he₁.trans he₂) hv₁ hv₂' ⟨v₂, hu₁, hu₂⟩
   case top.nest hv' _ _ _ _ hu hn _ _ =>
-    let l₁ := Lineage.end cmp $ Finmap.ids_def'.mpr ⟨_, hv'⟩
+    let l₁ := Lineage.end cmp $ Finmap.mem_ids_iff.mpr ⟨_, hv'⟩
     let l₂ := Lineage.nest hu.requires_lineage_to_target.some hn
     have hc := Reactor.uniqueIDs l₁ l₂
     cases cmp <;> contradiction
   case nest.top hn hu _ _ _ _ hv _ _ =>
-    let l₁ := Lineage.end cmp $ Finmap.ids_def'.mpr ⟨_, hv⟩
+    let l₁ := Lineage.end cmp $ Finmap.mem_ids_iff.mpr ⟨_, hv⟩
     let l₂ := Lineage.nest hu.preserves_lineage_to_target.some hn
     have hc := Reactor.uniqueIDs l₁ l₂
     cases cmp <;> contradiction
@@ -230,8 +230,21 @@ theorem Update.preserves_ne_cmp_or_id {cmp} {f : cmp.type → cmp.type} :
     -- have H := he _ _ ho
     sorry
 
+theorem Update.preserves_ne_cmp {cmp} {f : cmp.type → cmp.type} 
+    (u : σ₁ -[cmp:i f]→ σ₂) (hn : cmp' ≠ cmp := by exact (nomatch ·)) 
+    (hc : cmp ≠ .rtr := by exact (nomatch ·)) (hc' : cmp' ≠ .rtr := by exact (nomatch ·)) : 
+    σ₁.obj? cmp' i' = σ₂.obj? cmp' i' := by
+  sorry
+
+theorem Update.preserves_ne_id {cmp} {f : cmp.type → cmp.type} 
+    (u : σ₁ -[cmp:i f]→ σ₂) (hi : i' ≠ i) 
+    (hc : cmp ≠ .rtr := by exact (nomatch ·)) (hc' : cmp' ≠ .rtr := by exact (nomatch ·)) : 
+    σ₁.obj? cmp' i' = σ₂.obj? cmp' i' := by
+  sorry
+
 -- TODO: Cf. comment on EqModID.preserves_Equiv.
-theorem Update.preserves_Equiv {cmp} {u : cmp.type → cmp.type → Prop} : (σ₁ -[cmp;i u]→ σ₂) → (cmp ≠ .rtr) → σ₁ ≈ σ₂ := by
+theorem Update.equiv {cmp} {u : cmp.type → cmp.type → Prop} 
+    (u : σ₁ -[cmp;i u]→ σ₂) (hc : cmp ≠ .rtr := by exact (nomatch ·)) : σ₁ ≈ σ₂ := by
   sorry
 
 structure Mutation.rtrRel (cmp : Cmp) (cmpRel : (ID ⇉ cmp.type) → (ID ⇉ cmp.type) → Prop) (σ₁ σ₂ : Reactor) : Prop where
