src/ReactorModel/Determinism/ChangeStep.lean
@@ -1,0 +1,115 @@
+import ReactorModel.Determinism.ChangeEquiv
+
+open Classical
+
+namespace Execution
+
+theorem ChangeStep.preserves_progress (e : s₁ -[c]→ s₂) : s₁.progress = s₂.progress := by
+  cases e <;> rfl
+
+theorem ChangeStep.preserves_tag (e : s₁ -[c]→ s₂) : s₁.tag = s₂.tag := by
+  cases e <;> rfl
+
+theorem ChangeStep.preserves_rcns {i : ID} (e : s₁ -[c]→ s₂) :
+    s₁.rtr.obj? .rcn i = s₂.rtr.obj? .rcn i := by
+  cases e <;> first | rfl | simp [Reactor.Update.preserves_ne_cmp_or_id ‹_›]
+
+theorem ChangeStep.equiv (e : s₁ -[c]→ s₂) : s₁.rtr ≈ s₂.rtr := by
+  cases e 
+  case' port h, state h, action h => exact h.equiv
+  all_goals exact .refl 
+
+theorem ChangeStep.preserves_unchanged_port 
+    (e : s₁ -[c]→ s₂) (h : ¬c.obj.IsPort i := by exact (nomatch ·)) :
+    s₁.rtr.obj? .prt i = s₂.rtr.obj? .prt i := by
+  cases e
+  case port u => simp [Change.IsPort.iff_id_eq] at h; exact u.preserves_ne_id h
+  case' state u, action u => exact u.preserves_ne_cmp
+  all_goals rfl
+
+theorem ChangeStep.preserves_unchanged_state 
+    (e : s₁ -[c]→ s₂) (h : ¬c.obj.IsState i := by exact (nomatch ·)) : 
+    s₁.rtr.obj? .stv i = s₂.rtr.obj? .stv i := by
+  cases e
+  case state u => simp [Change.IsState.iff_id_eq] at h; exact u.preserves_ne_id h
+  case' action u, port u => exact u.preserves_ne_cmp
+  all_goals rfl
+
+theorem ChangeStep.preserves_unchanged_action 
+    (e : s₁ -[c]→ s₂) (h : ¬c.obj.IsAction i := by exact (nomatch ·)) : 
+    s₁.rtr.obj? .act i = s₂.rtr.obj? .act i := by
+  cases e 
+  case action u => simp [Change.IsAction.iff_id_eq] at h; exact u.preserves_ne_id h
+  case' state u, port u => exact u.preserves_ne_cmp 
+  all_goals rfl
+
+theorem ChangeStep.port_change {i : ID} (h : s₁.rtr.obj? .prt i = some p) :
+    (s₁ -[⟨rcn, .port i v⟩]→ s₂) → s₂.rtr.obj? .prt i = some { p with val := v }
+  | port u => by
+    have ⟨_, h₁, h₂⟩ := u.change'
+    injection h ▸ h₁ with h₁
+    simp [h₁, h₂]
+
+theorem ChangeStep.action_change {i : ID} (h : s₁.rtr.obj? .act i = some a) :
+    (s₁ -[⟨rcn, .action i t v⟩]→ s₂) → s₂.rtr.obj? .act i = some (schedule a t v)
+  | action u => by
+    have ⟨_, h₁, h₂⟩ := u.change'
+    injection h ▸ h₁ with h₁
+    simp [h₁, h₂]
+
+theorem ChangeStep.port_preserves_port_role {j : ID} 
+    (e : s₁ -[⟨rcn, .port i v⟩]→ s₂) (h : s₁.rtr.obj? .prt j = some p) :
+    ∃ v, s₂.rtr.obj? .prt j = some { p with val := v } :=
+  if hi : j = i
+  then ⟨v, hi ▸ e.port_change (hi ▸ h)⟩ 
+  else ⟨_, e.preserves_unchanged_port (Change.IsPort.iff_id_eq.not.mpr hi) ▸ h⟩ 
+      
+theorem ChangeStep.preserves_port_role {i : ID} 
+    (e : s₁ -[⟨rcn, c⟩]→ s₂) (h : s₁.rtr.obj? .prt i = some p) :
+    ∃ v, s₂.rtr.obj? .prt i = some { p with val := v } := by
+  cases c
+  case port => exact e.port_preserves_port_role h
+  all_goals
+    simp [←e.preserves_unchanged_port (i := i), h]
+    exists p.val
+
+theorem ChangeStep.preserves_same_action_at_unchanged_times
+    (e : s₁ -[⟨rcn, .action i t v⟩]→ s₂) (ht : t ≠ t') 
+    (ho₁ : s₁.rtr.obj? .act i = some a₁) (ho₂ : s₂.rtr.obj? .act i = some a₂) :
+    a₁ ⟨t', m⟩ = a₂ ⟨t', m⟩ := by
+  injection e.action_change ho₁ ▸ ho₂ with h
+  rw [←h, schedule_preserves_unchanged_time ht]  
+
+-- Note: `ho₁` and `e` imply `ho₂`.
+theorem ChangeStep.preserves_action_at_unchanged_times
+    (e : s₁ -[⟨rcn, c⟩]→ s₂) (hc : ¬c.IsActionAt i t) 
+    (ho₁ : s₁.rtr.obj? .act i = some a₁) (ho₂ : s₂.rtr.obj? .act i = some a₂) :
+  a₁ ⟨t, m⟩ = a₂ ⟨t, m⟩ := by
+  cases c
+  case action j t v =>
+    by_cases hi : i = j
+    case neg =>
+      have h := e.preserves_unchanged_action (i := i) (Change.IsAction.iff_id_eq.not.mpr hi) 
+      injection ho₁ ▸ ho₂ ▸ h with h
+      simp [h]
+    case pos =>
+      have ht := Change.not_IsActionAt_eq_ids_to_ne_time (hi ▸ hc)
+      exact e.preserves_same_action_at_unchanged_times ht (hi ▸ ho₁) (hi ▸ ho₂)
+  all_goals
+    injection ho₁ ▸ ho₂ ▸ e.preserves_unchanged_action (i := i) with h
+    simp [h]
+
+-- TODO: Check if this is still needed after cleaning up `ChangeListStep.equiv_changes_eq_result`.
+theorem ChangeStep.port_change_mem_rtr : 
+    (s -[⟨rcn, .port i v⟩]→ s') → ∃ p, s.rtr.obj? .prt i = some p
+  | .port u => u.obj?_target
+
+theorem ChangeStep.context_agnostic (e : s₁ -[c]→ s) (h : s₁.rtr = s₂.rtr) :
+  s₂ -[c]→ { s with tag := s₂.tag, progress := s₂.progress } := by
+  cases e
+  all_goals 
+    rw [h] at * 
+    constructor <;> assumption
+
+theorem ChangeStep.determinisic (e₁ : s -[c]→ s₁) (e₂ : s -[c]→ s₂) : s₁ = s₂ := by
+  cases e₁ <;> cases e₂ <;> simp <;> try apply Reactor.Update.unique' ‹_› ‹_› 
