src/ReactorModel/Execution/Schedule.lean
@@ -1,0 +1,42 @@
+import ReactorModel.Primitives
+
+namespace Execution
+
+-- NOTE: This does not constrain actions to have to be scheduled into the future.
+--       If we schedule something for the past, it doesn't matter, since that action value will never be read.
+--       But if the current tag has a microstep of 0, it is possible to schedule something for the current tag
+--       (in the `none` case).
+noncomputable def schedule (act : Time.Tag ⇉ Value) (t : Time) (v : Value) : Time.Tag ⇉ Value :=
+  match act.ids.filter (·.time = t) |>.max with
+  | none => act.update ⟨t, 0⟩ v
+  | some g => act.update ⟨t, g.microstep + 1⟩ v
+
+theorem schedule_preserves_unchanged_time (h : t ≠ t') : a ⟨t', m⟩ = (schedule a t v) ⟨t', m⟩ := by
+  unfold schedule
+  split
+  all_goals
+    apply Eq.symm
+    sorry
+    -- apply Finmap.update_ne
+    -- simp [h]
+
+theorem schedule_time_inj :
+  (∀ m, a₁ ⟨t, m⟩ = a₂ ⟨t, m⟩) → (schedule a₁ t v) ⟨t, m⟩ = (schedule a₂ t v) ⟨t, m⟩ := by
+  intro h
+  unfold schedule
+  cases a₁.ids.filter (·.time = t) |>.max <;>
+  cases a₂.ids.filter (·.time = t) |>.max
+  case' none.none, none.some =>
+    cases m
+    case zero => sorry -- simp [Finmap.update_self]
+    case succ => sorry -- simp [Finmap.update_ne, h]
+  case' some.some m₁ _, some.none m₁ =>
+    simp
+    by_cases hm : m₁.microstep + 1 = m
+    case pos => sorry -- simp [hm, Finmap.update_self]
+    case neg => 
+      sorry
+      -- have hm' : Time.Tag.mk t (m₁.microstep + 1) ≠ ⟨t, m⟩ := by simp [hm]
+      -- simp [Finmap.update_ne _ hm', h
+  
+end Execution
